fairis/heap_lang/lifting.v
@@ -196,28 +196,13 @@ Proof.
   iExists state_interp, (λ _, 0%nat ↦M ∅)%I, fork_post.
   iSplitR.
   { unfold config_wp. iIntros "!>!>" (???????) "?". done. }
-  (* iAssert (state_interp with "[Hgen Hmoda Hmodf Hmapa Hfuela HFR] Hfr [Hfuelf Hmapf]"). *)
-  (* { iFrame "Hmodf". unfold state_interp. simpl. iFrame. iExists {[ 0%nat := (live_roles Mdl s1) ]}, _. *)
-  (*   iSplitL "Hfuela"; first by rewrite /auth_fuel_is /= fmap_gset_to_gmap //. *)
-  (*   iSplitL "Hmapa"; first by rewrite /auth_mapping_is /= map_fmap_singleton //. *)
-  (*   iSplit; first done. *)
-  (*   iSplit; iPureIntro; [|split]. *)
-  (*   - intros ρ tid. rewrite lookup_gset_to_gmap_Some. *)
-  (*     setoid_rewrite lookup_singleton_Some. split; naive_solver. *)
-  (*   - intros tid Hlocs. rewrite lookup_singleton_ne //. compute in Hlocs. set_solver. *)
-  (*   - rewrite dom_gset_to_gmap. set_solver. } *)
   iSpecialize ("Hwp" with "Hσ Hmodf Hfr [Hfuelf Hmapf]").
-  { (* rewrite /has_fuels /frag_mapping_is /= map_fmap_singleton. iFrame. *)
-    
-    (* iAssert ([∗ set] ρ ∈ live_roles M s1, ρ ↦F (LM.(lm_fl) s1))%I with "[Hfuelf]" as "H". *)
-    
-    iAssert ([∗ map] ρ↦f ∈ gset_to_gmap (lm_fl LM s1) (live_roles M s1), 
+  { iAssert ([∗ map] ρ↦f ∈ gset_to_gmap (lm_fl LM s1) (live_roles M s1), 
   ρ ↦F f)%I with "[Hfuelf]" as "H".
     - unfold frag_fuel_is. setoid_rewrite map_fmap_singleton.
       rewrite -big_opM_own //; last first.
-      { intros ?. apply Hfevol. rewrite /gset_to_gmap in H.
-        apply fmap_empty_iff in H.
-        admit.                  (* TODO: Fix this... *) }
+      { intros Hm. apply dom_empty_iff_L in Hm. rewrite dom_gset_to_gmap in Hm.
+        done. }
       iApply (own_proper with "Hfuelf").
       rewrite -big_opM_auth_frag. f_equiv.
       rewrite big_opM_gset_to_gmap.
@@ -229,7 +214,6 @@ Proof.
   iSplitL "Hgen Hmoda Hmapa Hfuela HFR".
   { unfold state_interp. simpl. iFrame.
     iExists _, {[ 0%nat := (live_roles M s1) ]}, _.
-    (* iExists {[ 0%nat := (live_roles M s1) ]}, _, _. *)
     iSplit; first done.
     rewrite /auth_fuel_is /= fmap_gset_to_gmap //.
     rewrite /auth_mapping_is /= map_fmap_singleton //.
@@ -237,6 +221,7 @@ Proof.
     iPureIntro.
     split.
     { intros ρ Hρ Hin.
+      rewrite not_elem_of_dom in Hρ.
       rewrite lookup_gset_to_gmap_None in Hρ.
       set_solver. }
     split.
@@ -297,12 +282,10 @@ Proof.
       destruct tid as [|tid]; rewrite /from_locale /= in Hsome; by simplify_eq.
   - (* We need to prove that that the property is preserved *)
     destruct atr as [|atr' ℓ δ]; first by inversion Hvalex.
-    (* rewrite (trace_singleton_ends_in_inv _ _ Hendex); last exact unit. *)
     specialize (Hcontr ex' atr' tid ℓ).
     have H: trace_contract (trace_extend ex' tid (e, σ)) tid ex' by eexists.
     have H': trace_contract (trace_extend atr' ℓ δ) ℓ atr' by eexists.
     specialize (Hcontr H H') as Hvs. clear H H' Hcontr.
-    (* destruct Hvalex as (Hlm & Hlt & Hts). *)
     have H: trace_ends_in ex' (trace_last ex') by eexists.
     have H': trace_ends_in atr' (trace_last atr') by eexists.
     iApply (fupd_mask_weaken ∅); first set_solver. iIntros "_ !>".
@@ -322,7 +305,7 @@ Proof.
         apply from_locale_lookup =>//. }
       iDestruct (frag_mapping_same tid' rm with "Hrm H") as "%Hlk".
       { rewrite /auth_mapping_is. iPureIntro. by eapply no_locale_empty. }
-Admitted.
+Qed.
 
 Theorem simulation_adequacy Σ `(LM:LiveModel heap_lang M) `{!heapGpreS Σ LM} (s: stuckness) (e1 : expr) σ1 (s1: M) (FR: gset _):
   (* The model has finite branching *)
@@ -796,7 +779,6 @@ Lemma wp_step_model s tid ρ (f1 : nat) fs fr s1 s2 E e Φ :
   TCEq (to_val e) None →
   ρ ∉ dom fs →
   fmtrans M s1 (Some ρ) s2 →
-  (* live_roles _ s2 ⊆ live_roles _ s1 -> *)
   ▷ frag_model_is s1 -∗ ▷ has_fuels tid ({[ρ:=f1]} ∪ fmap S fs) -∗
   ▷ frag_free_roles_are fr -∗
   sswp s E e (λ e', frag_model_is s2 -∗ frag_free_roles_are fr -∗
@@ -834,8 +816,7 @@ Qed.
 
 Lemma wp_step_model_singlerole s tid ρ (f1 : nat) fr s1 s2 E e Φ :
   TCEq (to_val e) None →
-  fmtrans M s1 (Some ρ) s2 ->
-  (* live_roles _ s2 ⊆ live_roles _ s1 -> *)
+  fmtrans M s1 (Some ρ) s2 →
   ▷ frag_model_is s1 -∗ ▷ has_fuel tid ρ f1 -∗ ▷ frag_free_roles_are fr -∗
   sswp s E e (λ e', frag_model_is s2 -∗ frag_free_roles_are fr -∗
                     has_fuel tid ρ (LM.(lm_fl) s2) -∗
@@ -978,7 +959,6 @@ Proof.
   simplify_eq. iMod "Hclose" as "_". iMod "H" as "[Hfuels Hkont]".
   rewrite !app_nil_r.
   iDestruct "Hsi" as "(%&Hgh&Hmi)".
-  (* iDestruct "Hmi" as (??) "(?&?&?&?&?&?&%)". *)
   iMod (update_fuel_step with "Hfuels Hmi") as "H";
     [by intros X%dom_empty_inv_L | econstructor =>//; by apply fill_step | ].
   iModIntro.
@@ -989,184 +969,6 @@ Proof.
   repeat iSplit; try naive_solver.
   iApply "Hkont". iApply (has_fuels_proper with "Hfuels") =>//.
 Qed.
-
-(* Lemma wp_lift_pure_step_no_fork_remove_role rem s tid E E' Φ e1 e2 fs ϕ: *)
-(*   fs ≠ ∅ -> *)
-(*   rem ⊆ dom fs → *)
-(*   rem ∩ live_roles _ s = ∅ → *)
-(*   PureExec ϕ 1 e1 e2 -> *)
-(*   ϕ -> *)
-(*   (|={E}[E']▷=> frag_model_is s ∗ has_fuels_S tid fs ∗ *)
-(*                  (frag_model_is s -∗ (has_fuels tid (fs ⇂ (dom fs ∖ rem))) -∗ WP e2 @ tid; E {{ Φ }})) *)
-(*   ⊢ WP e1 @ tid; E {{ Φ }}. *)
-(* Proof. *)
-(*   intros NnO Hincl Hdisj Hpe Hϕ. *)
-(*   have Hps: pure_step e1 e2. *)
-(*   { specialize (Hpe Hϕ). by apply nsteps_once_inv in Hpe. } *)
-(*   iIntros "H". iApply wp_lift_step; eauto. *)
-(*   { destruct Hps as [Hred _]. specialize (Hred inhabitant). eapply reducible_not_val; eauto. } *)
-(*   iIntros (extr auxtr K tp1 tp2 σ1 Hvalex Hexend Hloc) "Hsi". *)
-(*   iMod "H". iMod fupd_mask_subseteq as "Hclose"; last iModIntro; first by set_solver. *)
-(*   iSplit; first by destruct Hps as [Hred _]. *)
-(*   iNext. iIntros (e2' σ2 efs Hpstep). *)
-(*   destruct Hps as [? Hdet]. specialize (Hdet _ _ _ _ Hpstep) as (?&?&?). *)
-(*   simplify_eq. iMod "Hclose" as "_". iMod "H" as "(Hmod & Hfuels & Hkont)". *)
-(*   rewrite !app_nil_r. *)
-(*   iDestruct "Hsi" as "(%&Hgh&Hmi)". *)
-(*   iDestruct (model_agree' with "Hmi Hmod") as %Heq. *)
-
-(*   iMod (update_no_step_enough_fuel _ _ rem with "Hfuels Hmi") as "H"; eauto; *)
-(*     [by intros X%dom_empty_inv_L | set_solver | econstructor =>//; by apply fill_step |]. *)
-(*   iModIntro. *)
-(*   iDestruct ("H") as (δ2 ℓ [Hlabels Hvse]) "[Hfuels Hmi]". *)
-(*   iExists δ2, ℓ. *)
-(*   rewrite /state_interp /=. *)
-(*   rewrite Hexend /=. list_simplifier. iFrame "Hgh Hmi". *)
-(*   repeat iSplit; last done. *)
-(*   - iPureIntro. destruct ℓ =>//. *)
-(*   - iPureIntro. destruct Hvse as (?&?&? )=>//. *)
-(*   - iPureIntro. destruct Hvse as (?&?&? )=>//. *)
-(*   - iApply ("Hkont" with "Hmod"). iApply (has_fuels_proper with "Hfuels") =>//. *)
-(* Qed. *)
-
-(* Lemma wp_lift_pure_step_no_fork_2 tid E E' Φ e1 e2 (fs: gmap (fmrole Mdl) nat) R ϕ: *)
-(*   R ≠ ∅ -> *)
-(*   PureExec ϕ 1 e1 e2 -> *)
-(*   ϕ -> *)
-(*   (forall (ρ: fmrole Mdl) (f: nat), fs !! ρ = Some f -> f > 0) -> *)
-(*   (|={E}[E']▷=> has_fuels tid R fs ∗ ((has_fuels tid R (fmap (λ (x: nat), (x - 1)%nat) fs)) -∗ WP e2 @ tid; E {{ Φ }})) *)
-(*   ⊢ WP e1 @ tid; E {{ Φ }}. *)
-(* Proof. *)
-
-(* Lemma wp_lift_pure_step_no_fork' fs tid E E' Φ e1 e2: *)
-(*   fs ≠ ∅ -> *)
-(*   PureExec True 1 e1 e2 -> *)
-(*   (|={E}[E']▷=> has_fuels_S tid fs ∗ ((has_fuels tid fs) -∗ WP e2 @ tid; E {{ Φ }})) *)
-(*   ⊢ WP e1 @ tid; E {{ Φ }}. *)
-(* Proof. *)
-(*   intros. by iApply wp_lift_pure_step_no_fork. *)
-(* Qed. *)
-
-(* Lemma wp_lift_pure_step_no_fork_singlerole tid E E' Φ e1 e2 ρ f φ: *)
-(*   PureExec φ 1 e1 e2 -> φ -> *)
-(*   (|={E}[E']▷=> has_fuel tid ρ (S f) ∗ ((has_fuel tid ρ f) -∗ WP e2 @ tid; E {{ Φ }})) *)
-(*   ⊢ WP e1 @ tid; E {{ Φ }}. *)
-(* Proof. *)
-(*   iIntros (??) "H". rewrite has_fuel_fuels_S. *)
-(*   iApply (wp_lift_pure_step_no_fork {[ ρ := f ]} {[ρ]}); eauto; last first. *)
-(*   rewrite has_fuel_fuels //. apply map_non_empty_singleton. *)
-(* Qed. *)
-
-(* TODO: We might want this *)
-(* Lemma wp_lift_pure_step_no_fork_take_step s1 s2 tid E E' fs1 fs2 fr1 Φ e1 e2 ρ φ: *)
-(*   PureExec φ 1 e1 e2 -> φ -> *)
-(*   valid_new_fuelmap (LM := LM) fs1 fs2 s1 s2 ρ -> *)
-(*   live_roles M s2 ∖ live_roles M s1 ⊆ fr1 → *)
-(*   M.(fmtrans) s1 (Some ρ) s2 -> *)
-(*   (|={E}[E']▷=> frag_model_is s1 ∗ has_fuels tid fs1 ∗ frag_free_roles_are fr1 ∗ *)
-(*                  (frag_model_is s2 -∗ frag_free_roles_are (fr1 ∖ (live_roles M s2 ∖ live_roles M s1)) *)
-(*                   -∗ (has_fuels tid fs2 -∗ WP e2 @ tid; E {{ Φ }}))) *)
-(*   ⊢ WP e1 @ tid; E {{ Φ }}. *)
-(* Proof. *)
-(*   iIntros (Hpe Hφ Hval Hfr Htrans). *)
-(*   have Hps: pure_step e1 e2. *)
-(*   { specialize (Hpe Hφ). by apply nsteps_once_inv in Hpe. } *)
-(*   iIntros "Hkont". *)
-(*   iApply wp_lift_step; eauto. *)
-(*   { destruct (pure_step_safe _ e2 Hps inhabitant) as (?&?&?&?). by eapply val_stuck. } *)
-
-(*   iIntros (extr auxtr K tp1 tp2 σ1 Hvalex Hexend Hloc) "Hsi". *)
-(*   iMod "Hkont". iMod fupd_mask_subseteq as "Hclose"; last iModIntro; first by set_solver. *)
-(*   iSplit; first by destruct Hps as [Hred _]. *)
-(*   iNext. iIntros (e2' σ2 efs Hpstep). *)
-(*   destruct Hps as [? Hdet]. specialize (Hdet _ _ _ _ Hpstep) as (?&?&?). *)
-(*   simplify_eq. iMod "Hclose" as "_". iMod "Hkont" as "(Hmod&Hfuels&Hfr&Hkont)". *)
-(*   rewrite !app_nil_r. *)
-(*   iDestruct "Hsi" as "(%&Hgh&Hmi)". simpl. *)
-(*   iDestruct (model_agree' with "Hmi Hmod") as %Hmeq. *)
-
-(*   iMod (update_step_still_alive _ _ _ _ σ1 σ1 with "Hfuels Hmod Hmi Hfr") as "H"; eauto. *)
-(*   { rewrite Hexend. eauto. } *)
-(*   { econstructor =>//. *)
-(*     - rewrite Hexend //=. *)
-(*     - by apply fill_step. } *)
-(*   { rewrite Hmeq. apply Hval. } *)
-(*   iModIntro. iDestruct "H" as (δ2 ℓ [Hlabels Hvse]) "(Hfuels&Hmod&Hmi&Hfr)". *)
-(*   iExists δ2, ℓ. *)
-(*   rewrite Hexend /=. list_simplifier. iFrame "Hgh Hmi". *)
-(*   repeat iSplit; last done. *)
-(*   - iPureIntro. destruct ℓ =>//. *)
-(*   - iPureIntro. destruct Hvse as (?&?&? )=>//. *)
-(*   - iPureIntro. destruct Hvse as (?&?&? )=>//. *)
-(*   - by iSpecialize ("Hkont" with "Hmod Hfr Hfuels"). *)
-(* Qed. *)
-
-(* Lemma wp_lift_pure_step_no_fork_singlerole_take_step s1 s2 tid E E' (f1 f2: nat) fr Φ e1 e2 ρ φ: *)
-(*   PureExec φ 1 e1 e2 -> φ -> *)
-(*   live_roles _ s2 ⊆ live_roles _ s1 -> *)
-(*   (f2 ≤ LM.(lm_fl) s2)%nat -> M.(fmtrans) s1 (Some ρ) s2 -> *)
-(*   (|={E}[E']▷=> frag_model_is s1 ∗ frag_free_roles_are fr ∗ has_fuel tid ρ f1 ∗ *)
-(*    (frag_model_is s2 -∗ frag_free_roles_are fr -∗ (if decide (ρ ∈ live_roles M s2) then has_fuel tid ρ f2 else tid ↦M ∅) -∗ *)
-(*                                WP e2 @ tid; E {{ Φ }})) *)
-(*   ⊢ WP e1 @ tid; E {{ Φ }}. *)
-(* Proof. *)
-(*   iIntros (Hpe Hφ Hroles Hfl Hmdl). *)
-(*   rewrite has_fuel_fuels. *)
-(*   iIntros "H". *)
-(*   iApply (wp_lift_pure_step_no_fork_take_step _ _ _ _ _ {[ρ := f1]} *)
-(*          (if decide (ρ ∈ live_roles M s2) then {[ρ := f2]} else ∅) fr  with "[H]"); eauto. *)
-(*   - repeat split. *)
-(*     + intros ?. rewrite decide_True //. rewrite lookup_singleton //=. *)
-(*     + destruct (decide (ρ ∈ live_roles _ s2)); set_solver. *)
-(*     + set_solver. *)
-(*     + intros ρ' Hdom. destruct (decide (ρ ∈ live_roles M s2)); set_solver. *)
-(*     + intros ρ' Hneq Hin. destruct (decide (ρ ∈ live_roles M s2)); set_solver. *)
-(*     + destruct (decide (ρ ∈ live_roles M s2)); set_solver. *)
-(*     + destruct (decide (ρ ∈ live_roles M s2)); set_solver. *)
-(*   - set_solver. *)
-(*   - iMod "H". do 2 iModIntro. iMod "H" as "(Hmod&Hfr&Hfuels&Hkont)". iModIntro. *)
-(*     iFrame "Hmod Hfr Hfuels". iIntros "Hmod Hfr Hfuels". iApply ("Hkont" with "Hmod [Hfr] [Hfuels]"). *)
-(*     + replace (fr ∖ (live_roles M s2 ∖ live_roles M s1)) with fr; [done|set_solver]. *)
-(*     + destruct (decide (ρ ∈ live_roles M s2)). *)
-(*       * rewrite -has_fuel_fuels //. *)
-(*       * iDestruct "Hfuels" as "[Hf _]". rewrite dom_empty_L //. *)
-(* Qed. *)
-
-(* Lemma wp_lift_pure_step_no_fork_singlerole' tid E E' Φ e1 e2 ρ f: *)
-(*   PureExec True 1 e1 e2 -> *)
-(*   (|={E}[E']▷=> has_fuel tid ρ (S f) ∗ ((has_fuel tid ρ f) -∗ WP e2 @ tid; E {{ Φ }})) *)
-(*   ⊢ WP e1 @ tid; E {{ Φ }}. *)
-(* Proof. *)
-(*   iIntros (?) "H". rewrite has_fuel_fuels_S. *)
-(*   iApply (wp_lift_pure_step_no_fork' {[ ρ := f ]} {[ρ]}); last first. *)
-(*   rewrite has_fuel_fuels //. apply map_non_empty_singleton. *)
-(* Qed. *)
-
-(* (** Fork: Not using Texan triples to avoid some unnecessary [True] *) *)
-(* Lemma wp_fork_nostep s tid E e Φ R1 R2 fs (Hdisj: R1 ## R2) (Hnemp: fs ≠ ∅): *)
-(*   R1 ∪ R2 = dom fs -> *)
-(*   (∀ tid', ▷ (has_fuels tid' (fs ⇂ R2) -∗ WP e @ s; tid'; ⊤ {{ _, tid' ↦M ∅ }})) -∗ *)
-(*      ▷ (has_fuels tid (fs ⇂ R1) ={E}=∗ Φ (LitV LitUnit)) -∗ *)
-(*      has_fuels_S tid fs -∗ WP Fork e @ s; tid; E {{ Φ }}. *)
-(* Proof. *)
-(*   iIntros (Hunioneq) "He HΦ Htid". iApply wp_lift_atomic_head_step; [done|]. *)
-(*   iIntros (extr auxtr K tp1 tp2 σ1 Hvalex Hexend Hloc) "(% & Hsi & Hmi)". *)
-(*   iMod (update_fork_split R1 R2 _ *)
-(*        (tp1 ++ ectx_language.fill K (Val $ LitV LitUnit) :: tp2 ++ [e]) fs _ _ _ e _ σ1 with "Htid Hmi") as *)
-(*        (δ2) "(Hfuels2 & Hfuels1 & Hσ & %Hvse)" => //. *)
-(*   { rewrite -Hloc. rewrite -(language.locale_fill _ _ K). econstructor 1 =>//. *)
-(*     apply fill_step, head_prim_step. econstructor. } *)
-(*   { list_simplifier. exists (tp1 ++ fill K #() :: tp2). split; first by list_simplifier. *)
-(*     rewrite !app_length //=. } *)
-(*   iModIntro. iSplit. iPureIntro; first by eauto. iNext. *)
-(*   iIntros (e2 σ2 efs Hstep). *)
-(*   have [-> [-> ->]] : σ2 = σ1 ∧ efs = [e] ∧ e2 = Val $ LitV LitUnit by inv_head_step. *)
-(*   iMod ("HΦ" with "Hfuels1") as "HΦ". iModIntro. iExists δ2, (Silent_step tid). iFrame. *)
-(*   rewrite Hexend /=. iFrame "Hsi". *)
-(*   iSplit; first by iPureIntro. *)
-(*   iSplit; [|done]. *)
-(*   iApply "He". by list_simplifier. *)
-(* Qed. *)
 
 (** Heap *)
 (** The usable rules for [allocN] stated in terms of the [array] proposition
@@ -1232,44 +1034,7 @@ Proof.
   + iApply (heap_array_to_seq_meta with "Hm"). by rewrite replicate_length.
 Qed.
 
-(* Lemma wp_allocN_seq_nostep' s tid E v n fs: *)
-(*   fs ≠ ∅ -> *)
-(*   0 < n → *)
-(*   {{{ has_fuels_S tid fs }}} AllocN (Val $ LitV $ LitInt $ n) (Val v) @ s; tid; E *)
-(*   {{{ l, RET LitV (LitLoc l); has_fuels tid fs ∗ [∗ list] i ∈ seq 0 (Z.to_nat n), *)
-(*       (l +ₗ (i : nat)) ↦ v ∗ meta_token (l +ₗ (i : nat)) ⊤ }}}. *)
-(* Proof. *)
-(*   iIntros (HnO Hn Φ) "HfuelS HΦ". iApply wp_lift_atomic_head_step_no_fork; auto. *)
-(*   iIntros (extr auxtr K tp1 tp2 σ1 Hvalex Hexend Hloc) "(% & Hsi & Hmi)". *)
-(*   iModIntro; iSplit; first by eauto. *)
-(*   iIntros (e2 σ2 efs Hstep). iNext. *)
-(*   inv_head_step. *)
-(*   iMod (gen_heap_alloc_big _ (heap_array l (replicate (Z.to_nat n) v)) with "Hsi") *)
-(*     as "(Hsi & Hl & Hm)". *)
-(*   { apply heap_array_map_disjoint. *)
-(*     rewrite replicate_length Z2Nat.id ?Hexend; auto with lia. } *)
-(*   iMod (update_no_step_enough_fuel _ _ ∅ with "HfuelS Hmi") as (δ2 ℓ) "([%Hlabel %Hvse] & Hfuel & Hmi)" =>//. *)
-(*   { by intros ?%dom_empty_inv_L. } *)
-(*   { set_solver. } *)
-(*   { rewrite Hexend. apply head_locale_step. by econstructor. } *)
-(*   iModIntro; iExists δ2, ℓ. *)
-(*   rewrite Hexend //=. iFrame "Hmi Hsi". *)
-(*   repeat iSplit =>//. *)
-(*   iApply "HΦ". iSplitL "Hfuel". *)
-(*   { iApply (has_fuels_proper with "Hfuel") =>//. *)
-(*     rewrite map_filter_id //. intros ???%elem_of_dom_2; set_solver. } *)
-(*   iApply big_sepL_sep. iSplitL "Hl". *)
-(*   + by iApply heap_array_to_seq_mapsto. *)
-(*   + iApply (heap_array_to_seq_meta with "Hm"). by rewrite replicate_length. *)
-(* Qed. *)
-
-(* Lemma wp_alloc_nostep s tid E v fs : *)
-(*   fs ≠ ∅ -> *)
-(*   {{{ has_fuels_S tid fs }}} Alloc (Val v) @ s; tid; E {{{ l, RET LitV (LitLoc l); l ↦ v ∗ meta_token l ⊤ ∗ has_fuels tid fs }}}. *)
-(* Proof. *)
-(*   iIntros (? Φ) "HfuelS HΦ". iApply (wp_allocN_seq_nostep with "HfuelS"); auto with lia. *)
-(*   iIntros "!>" (l) "/= (? & ? & _)". rewrite loc_add_0. by iApply "HΦ"; iFrame. *)
-(* Qed. *)
+(* TODO: Bumped up to this point. *)
 
 Lemma wp_choose_nat_nostep s tid E fs :
   fs ≠ ∅ ->
